use spec.agile.hash in sha2-vec

code/sha2-vec/Hacl.SHA2.Scalar32.fst
@@ -15,7 +15,7 @@ open Hacl.Spec.SHA2.Vec
 open Hacl.Impl.SHA2.Generic
 
 module ST = FStar.HyperStack.ST
-module Spec = Hacl.Spec.SHA2
+module Spec = Spec.Agile.Hash
 module SpecVec = Hacl.Spec.SHA2.Vec
 
 
@@ -29,9 +29,10 @@ let sha256_update1 b hash = update #SHA2_256 #M32 b hash
 
 val sha256: hash:lbuffer uint8 32ul -> len:size_t -> b:lbuffer uint8 len ->
   Stack unit
-  (requires fun h0 -> live h0 b /\ live h0 hash /\ disjoint hash b)
+  (requires fun h0 -> v len <= max_input_length SHA2_256 /\
+    live h0 b /\ live h0 hash /\ disjoint hash b)
   (ensures  fun h0 _ h1 -> modifies (loc hash) h0 h1 /\
-    as_seq h1 hash == Spec.hash #SHA2_256 (v len) (as_seq h0 b))
+    as_seq h1 hash == Spec.hash SHA2_256 (as_seq h0 b))
 
 let sha256 h len b =
   let h0 = ST.get() in
@@ -39,7 +40,7 @@ let sha256 h len b =
   let h = ntup1 h in
   hash #SHA2_256 #M32 (sha256_update1 <: update_vec_t SHA2_256 M32) h len b;
   let h1 = ST.get() in
-  Hacl.Spec.SHA2.Equiv.hash_lemma #SHA2_256 #M32 (v len) (as_seq_multi h0 b);
+  Hacl.Spec.SHA2.Equiv.hash_agile_lemma #SHA2_256 #M32 (v len) (as_seq_multi h0 b);
   let hash0 = tup1 h in
   assert ((as_seq_multi h1 h).(|0|) == as_seq h1 hash0)
 
@@ -52,9 +53,10 @@ let sha512_update1 b hash = update #SHA2_512 #M32 b hash
 
 val sha512: hash:lbuffer uint8 64ul -> len:size_t -> b:lbuffer uint8 len ->
   Stack unit
-  (requires fun h0 -> live h0 b /\ live h0 hash /\ disjoint hash b)
+  (requires fun h0 -> v len <= max_input_length SHA2_512 /\
+    live h0 b /\ live h0 hash /\ disjoint hash b)
   (ensures  fun h0 _ h1 -> modifies (loc hash) h0 h1 /\
-    as_seq h1 hash == Spec.hash #SHA2_512 (v len) (as_seq h0 b))
+    as_seq h1 hash == Spec.hash SHA2_512 (as_seq h0 b))
 
 let sha512 h len b =
   let h0 = ST.get() in
@@ -62,6 +64,6 @@ let sha512 h len b =
   let h = ntup1 h in
   hash #SHA2_512 #M32 (sha512_update1 <: update_vec_t SHA2_512 M32) h len b;
   let h1 = ST.get() in
-  Hacl.Spec.SHA2.Equiv.hash_lemma #SHA2_512 #M32 (v len) (as_seq_multi h0 b);
+  Hacl.Spec.SHA2.Equiv.hash_agile_lemma #SHA2_512 #M32 (v len) (as_seq_multi h0 b);
   let hash0 = tup1 h in
   assert ((as_seq_multi h1 h).(|0|) == as_seq h1 hash0)
