code/sha2-vec/Hacl.SHA2.Vec128.fst
@@ -15,7 +15,7 @@ open Hacl.Spec.SHA2.Vec
 open Hacl.Impl.SHA2.Generic
 
 module ST = FStar.HyperStack.ST
-module Spec = Hacl.Spec.SHA2
+module Spec = Spec.Agile.Hash
 module SpecVec = Hacl.Spec.SHA2.Vec
 
 
@@ -29,12 +29,13 @@ let sha256_update4 b hash = update #SHA2_256 #M128 b hash
 
 val sha256_4 (r0 r1 r2 r3: lbuffer uint8 32ul) (len:size_t) (b0 b1 b2 b3: lbuffer uint8 len) :
   Stack unit
-  (requires fun h0 -> live4 h0 b0 b1 b2 b3 /\ live4 h0 r0 r1 r2 r3 /\ internally_disjoint4 r0 r1 r2 r3)
+  (requires fun h0 -> v len <= max_input_length SHA2_256 /\
+    live4 h0 b0 b1 b2 b3 /\ live4 h0 r0 r1 r2 r3 /\ internally_disjoint4 r0 r1 r2 r3)
   (ensures  fun h0 _ h1 -> modifies (loc r0 |+| loc r1 |+| loc r2 |+| loc r3) h0 h1 /\
-    as_seq h1 r0 == Spec.hash #SHA2_256 (v len) (as_seq h0 b0) /\
-    as_seq h1 r1 == Spec.hash #SHA2_256 (v len) (as_seq h0 b1) /\
-    as_seq h1 r2 == Spec.hash #SHA2_256 (v len) (as_seq h0 b2) /\
-    as_seq h1 r3 == Spec.hash #SHA2_256 (v len) (as_seq h0 b3))
+    as_seq h1 r0 == Spec.hash SHA2_256 (as_seq h0 b0) /\
+    as_seq h1 r1 == Spec.hash SHA2_256 (as_seq h0 b1) /\
+    as_seq h1 r2 == Spec.hash SHA2_256 (as_seq h0 b2) /\
+    as_seq h1 r3 == Spec.hash SHA2_256 (as_seq h0 b3))
 
 let sha256_4 r0 r1 r2 r3 len b0 b1 b2 b3 =
   let h0 = ST.get() in
@@ -47,7 +48,7 @@ let sha256_4 r0 r1 r2 r3 len b0 b1 b2 b3 =
   loc_multi4 rb;
   hash #SHA2_256 #M128 sha256_update4 rb len ib;
   let h1 = ST.get() in
-  Hacl.Spec.SHA2.Equiv.hash_lemma #SHA2_256 #M128 (v len) (as_seq_multi h0 ib);
+  Hacl.Spec.SHA2.Equiv.hash_agile_lemma #SHA2_256 #M128 (v len) (as_seq_multi h0 ib);
   assert ((as_seq_multi h1 rb).(|0|) == as_seq h1 r0);
   assert ((as_seq_multi h1 rb).(|1|) == as_seq h1 r1);
   assert ((as_seq_multi h1 rb).(|2|) == as_seq h1 r2);
