code/sha2-vec/Hacl.Spec.SHA2.EquivScalar.fsti
@@ -9,9 +9,5 @@ open Hacl.Spec.SHA2
 
 #set-options "--z3rlimit 50 --fuel 0 --ifuel 0"
 
-let max_size_t_lt_max_input_length (a:sha2_alg) : Lemma (max_size_t < max_input_length a) =
-  Math.Lemmas.pow2_lt_compat 61 32;
-  Math.Lemmas.pow2_lt_compat 125 32
-
-val hash_lemma: #a:sha2_alg -> len:size_nat -> b:lseq uint8 len ->
-  Lemma (max_size_t_lt_max_input_length a; hash #a len b == Spec.Agile.Hash.hash a b)
+val hash_agile_lemma: #a:sha2_alg -> len:size_nat{len <= max_input_length a} -> b:lseq uint8 len ->
+  Lemma (hash #a len b == Spec.Agile.Hash.hash a b)
